\documentclass[12pt]{article}
\usepackage{amsmath}
\usepackage{ amssymb }
\usepackage{breqn}
\begin{document}



\section{Linearisation}

So we do a linearisation for a pertubation on still water so (keep $O(\epsilon)$ terms)

\[h(x,t) = H + \epsilon\eta(x,t)\]
\[h = H + \epsilon\eta\]

\[u(x,t) = 0 + \epsilon v(x,t)\]

\[u =  \epsilon v\]

We start with $G$

\[G = uh - \left(\frac{h^3}{3} u_x\right)_x\]

\[G = \left(\epsilon v\right)\left(H + \epsilon\eta\right) - h^2h_x u_x  - \left(\frac{h^3}{3} u_{xx}\right)\]

\[G = \epsilon v H + \epsilon^2 v \eta  - \left(H + \epsilon\eta\right)^2 \epsilon\eta_x \epsilon v_x  - \left( \frac{H + \epsilon\eta^3}{3} \right) \epsilon v_{xx}\]

\[G = \epsilon v H   - \left( \frac{H + \epsilon\eta}{3} \right)^3 \epsilon v_{xx}\]

\[G = \epsilon v H   -  \frac{H^3}{3} \epsilon v_{xx}\]

Mass equation

\[h_t + uh_x + u_xh = 0\]
 

\[\left(H + \epsilon\eta\right)_t + \epsilon v\left(H + \epsilon\eta\right)_x + \epsilon v_x\left(H + \epsilon\eta\right) = 0\]

\[\epsilon\eta_t + \epsilon H v_x = 0\]

Momentum equation:

\[G_t + \left(Gu + \frac{gh^2}{2} - \frac{2h^3}{3} u_x u_x\right)_x = 0\]

\[\left(uh - \left(\frac{h^3}{3} u_x\right)_x\right)_t + \left(\left(uh - \left(\frac{h^3}{3} u_x\right)_x\right)u + \frac{gh^2}{2} - \frac{2h^3}{3} u_x u_x\right)_x = 0\]

\[\left(uh\right)_t - \left(\frac{h^3}{3} u_x\right)_{xt} + \left(u^2h - u\left(\frac{h^3}{3} u_x\right)_x + \frac{gh^2}{2} - \frac{2h^3}{3} u_x u_x\right)_x = 0\]

\[u_th + uh_t- \left(\frac{h^3}{3} u_x\right)_{xt} + \left(u^2h\right)_x + \left(- u\left(\frac{h^3}{3} u_x\right)_x \right)_x + \left(\frac{gh^2}{2} \right)_x + \left( - \frac{2h^3}{3} u_x u_x\right)_x = 0\]

\[H\epsilon v_t - \left(h^2h_x u_x +\frac{h^3}{3} u_{xx} \right)_{t} + \left(u^2h\right)_x + \left(- u\left(\frac{h^3}{3} u_x\right)_x \right)_x + \left(\frac{gh^2}{2} \right)_x + \left( - \frac{2h^3}{3} u_x u_x\right)_x = 0\]

\[H\epsilon v_t - \frac{H^3}{3}\epsilon v_{xxt} + \left(u^2h\right)_x + \left(- u\left(\frac{h^3}{3} u_x\right)_x \right)_x + \left(\frac{gh^2}{2} \right)_x + \left( - \frac{2h^3}{3} u_x u_x\right)_x = 0\]

\[H\epsilon v_t - \frac{H^3}{3}\epsilon v_{xxt} + 2uu_xh + u^2h_x + \left(- u\left(\frac{h^3}{3} u_x\right)_x \right)_x + \left(\frac{gh^2}{2} \right)_x + \left( - \frac{2h^3}{3} u_x u_x\right)_x = 0\]

\[H\epsilon v_t - \frac{H^3}{3}\epsilon v_{xxt} + \left(- u\left(\frac{h^3}{3} u_x\right)_x \right)_x + \left(\frac{gh^2}{2} \right)_x + \left( - \frac{2h^3}{3} u_x u_x\right)_x = 0\]

\[H\epsilon v_t - \frac{H^3}{3}\epsilon v_{xxt} + \left(- u\left(h^2h_xu_x + \frac{h^3}{3} u_{xx}\right)\right)_x + \left(\frac{gh^2}{2} \right)_x + \left( - \frac{2h^3}{3} u_x u_x\right)_x = 0\]

\[H\epsilon v_t - \frac{H^3}{3}\epsilon v_{xxt} + \left(- uh^2h_xu_x -u \frac{h^3}{3} u_{xx}\right)_x + \left(\frac{gh^2}{2} \right)_x + \left( - \frac{2h^3}{3} u_x u_x\right)_x = 0\]

\[H\epsilon v_t - \frac{H^3}{3}\epsilon v_{xxt} + \left(- uh^2h_xu_x \right)_x + \left(-u \frac{h^3}{3} u_{xx}\right)_x + \left(\frac{gh^2}{2} \right)_x + \left( - \frac{2h^3}{3} u_x u_x\right)_x = 0\]

\[H\epsilon v_t - \frac{H^3}{3}\epsilon v_{xxt} + \left(- u_xh^2h_xu_x \right)  + \left(- uhh_xh_xu_x \right)_x + \left(- uh^2h_{xx}u_x \right) + \left(- uh^2h_xu_{xx} \right) + \left(-u \frac{h^3}{3} u_{xx}\right)_x + \left(\frac{gh^2}{2} \right)_x + \left( - \frac{2h^3}{3} u_x u_x\right)_x = 0\]

\[H\epsilon v_t - \frac{H^3}{3}\epsilon v_{xxt}  + \left(-u \frac{h^3}{3} u_{xx}\right)_x + \left(\frac{gh^2}{2} \right)_x + \left( - \frac{2h^3}{3} u_x u_x\right)_x = 0\]

\[H\epsilon v_t - \frac{H^3}{3}\epsilon v_{xxt}  - \epsilon v \frac{(h + \epsilon \eta)^3}{3} \epsilon v_{xxx} + \left(\frac{gh^2}{2} \right)_x + \left( - \frac{2h^3}{3} u_x u_x\right)_x = 0\]

\[H\epsilon v_t - \frac{H^3}{3}\epsilon v_{xxt}  + \left(\frac{gh^2}{2} \right)_x  = 0\]

\[H\epsilon v_t - \frac{H^3}{3}\epsilon v_{xxt}  + gH\epsilon \eta_x  = 0\]

So we have

\[G = \epsilon v H   -  \frac{H^3}{3} \epsilon v_{xx}\]

\[\epsilon\eta_t + \epsilon H v_x = 0\]

\[H\epsilon v_t - \frac{H^3}{3}\epsilon v_{xxt}  + gH\epsilon \eta_x  = 0\]

using u's instead of v's, incorporating epsilon into its relevant term and using h instead of H we get. 


\[G = uh  -  \frac{h^3}{3} u_{xx}\]

\[\eta_t + h u_x = 0\]

\[h u_t - \frac{h^3}{3} u_{xxt}  + gh \eta_x  = 0\]


\end{document}
