\documentclass[12pt]{article}
\usepackage{amsmath}
\usepackage{ amssymb }
\usepackage{breqn}
\begin{document}

\

\[\mathcal{C}_2 = \frac{ 2\cos\left(k\Delta x\right) - 2 }{\Delta x^2}\]


\[\mathcal{C}_4 = \frac{-2\cos\left(2k\Delta x\right) + 32\cos\left(k\Delta x\right)  - 30 }{12\Delta x^2}\]


We define:
\[\mathcal{G} = \left[H -\frac{H^3}{3} \mathcal{C}\right]\]


\[G_j = \mathcal{G}u_j\]



\[\mathcal{M}_3= \frac{26  -2\cos\left(k\Delta x\right)}{24}\]

We again will suppress order subscripts further on, but we also have $\mathcal{M}_1 = \mathcal{M}_2 = 1$.
\subsubsection{Reconstruction}


So we define $\mathcal{R}^+_1 =  e^{ik\Delta x}$ and $\mathcal{R}^-_1 =  1$. 

So we have that
\[\mathcal{R}_2^- = 1  + \frac{i\sin\left(k\Delta x\right)}{2}\]
\[\mathcal{R}_2^+ = e^{ik\Delta x}\left(1  - \frac{i\sin\left(k\Delta x\right)}{2} \right)\]

\[R_3^-= \frac{\mathcal{M}_3}{6}\left[5 +  - e^{-ik\Delta x} + 2e^{ik\Delta x} \right]\]


\[R_3^+= \frac{\mathcal{M}_3 e^{ik\Delta x }}{6}\left[5 + 2e^{-ik\Delta x} - e^{ik\Delta x} \right]\] 

\[R^u_2 = \frac{e^{ik\Delta x } - 1}{2} \]

\[R^u_3 = \frac{-3e^{2ik\Delta x } + 27e^{ik\Delta x } + 27 - 3e^{-ik\Delta x }}{48}\]


\[\mathcal{F}^{h,u} = H\mathcal{R}^u\]

\[\mathcal{F}^{h,h} = -\dfrac{ \sqrt{gH}}{ 2} \left [ \mathcal{R}^+- \mathcal{R}^- \right ]\]

\[\mathcal{F}^{u,u} = - \dfrac{ \sqrt{gH}}{ 2} \mathcal{G} \left [ \mathcal{R}^+ \ -  \mathcal{R}^-  \right ]\]

\[\mathcal{F}^{u,h} = \dfrac{ gH \mathcal{R}^- + gH \mathcal{R}^+}{ 2}\]


Defining $\mathcal{D} = 1 -e^{-ik\Delta x}$

\end{document}
