\documentclass[12pt]{article}
\usepackage{amsmath}
\usepackage{ amssymb }
\usepackage{breqn}
\begin{document}

\section{All Definitions for Numerical Versions}
\[\mathcal{C}_2 = \frac{ 2\cos\left(k\Delta x\right) - 2 }{\Delta x^2}\]

\[\mathcal{C}_4 = \frac{-2\cos\left(2k\Delta x\right) + 32\cos\left(k\Delta x\right)  - 30 }{12\Delta x^2}\]

\[\mathcal{G} = \left[H -\frac{H^3}{3} \mathcal{C}\right]\]

\[\mathcal{M}_3= \frac{26  -2\cos\left(k\Delta x\right)}{24}\]
\[\mathcal{M}_1 = \mathcal{M}_2 = 1\]

\[\mathcal{R}^+_1 =  e^{ik\Delta x} \quad , \quad\mathcal{R}^-_1 =  1\]

\[\mathcal{R}_2^- = 1  + \frac{i\sin\left(k\Delta x\right)}{2}\]
\[\mathcal{R}_2^+ = e^{ik\Delta x}\left(1  - \frac{i\sin\left(k\Delta x\right)}{2} \right)\]

\[\mathcal{R}_3^-= \frac{\mathcal{M}_3}{6}\left[5 +  - e^{-ik\Delta x} + 2e^{ik\Delta x} \right]\]

\[\mathcal{R}_3^+= \frac{\mathcal{M}_3 e^{ik\Delta x }}{6}\left[5 + 2e^{-ik\Delta x} - e^{ik\Delta x} \right]\] 

\[\mathcal{R}^u_2 = \frac{e^{ik\Delta x } + 1}{2} \]

\[\mathcal{R}^u_3 = \frac{-3e^{2ik\Delta x } + 27e^{ik\Delta x } + 27 - 3e^{-ik\Delta x }}{48}\]


\[\mathcal{F}^{h,u} = H\mathcal{R}^u\]

\[\mathcal{F}^{h,h} = -\dfrac{ \sqrt{gH}}{ 2} \left [ \mathcal{R}^+- \mathcal{R}^- \right ]\]

\[\mathcal{F}^{u,u} = - \dfrac{ \sqrt{gH}}{ 2} \mathcal{G} \left [ \mathcal{R}^+ \ -  \mathcal{R}^-  \right ]\]

\[\mathcal{F}^{u,h} = \dfrac{ gH \mathcal{R}^- + gH \mathcal{R}^+}{ 2}\]


$\mathcal{D} = 1 -e^{-ik\Delta x}$

\section{Taylor Expansions Of Analytic Values }
We denote exact/analytic version with a subscript $a$

\[\mathcal{G}_a = H + \frac{H^3}{3}k^2\]

\[\mathcal{M}_a = 1 + \frac{1}{24} (k\Delta x)^2 + \frac{7}{5760} (k\Delta x)^4 + O(x^{6}) \]

\[\mathcal{R}_a^+ = \mathcal{R}_a^-=\mathcal{R}_a = 1 + \frac{i}{2}k\Delta x   - \frac{1}{8}k^2\Delta x^2 - \frac{i}{48}k^3\Delta x^3 + O(x^{4})\]

For the fluxes I think its best to group the $ \frac{1}{\Delta x}\mathcal{D}\mathcal{F}$ because $ \frac{1}{\Delta x}\mathcal{D}\mathcal{F}$ approximates the derivative of the flux term. Which gives the following coefficients. 
\[\mathcal{D}_a\mathcal{F}^{h,u}_a = ikH\]
\[\mathcal{D}_a\mathcal{F}^{h,h}_a = 0\]
\[\mathcal{D}_a\mathcal{F}^{u,h}_a = ikgH\]
\[\mathcal{D}_a\mathcal{F}^{u,u}_a = 0\]

\section{Taylor Expansions Of First Order Values }

\[\mathcal{G}_1 = H +\frac{H^3}{3} k^2 -\frac{H^3 k^4(\Delta x)^2}{36} + O(x^{4})\]
\[\mathcal{M}_1 = 1\]

\[\mathcal{R}^-_1 =  1\]

\[\mathcal{R}^+_1 = 1 + i k\Delta x  - \frac{1}{2} (k\Delta x)^2 - \frac{i}{3!} (k\Delta x)^3 + \frac{1}{4!} (k\Delta x)^4 +  O((k\Delta x)^5)\]

\[\mathcal{R}^u_1 = 1 + \frac{i}{2}k\Delta x - \frac{1}{4} (k \Delta x)^2 - \frac{i}{12} (k \Delta x)^3 +  O( \Delta x^4)\]

\[\mathcal{D}\mathcal{F}^{h,u}_1 = Hik\Delta x  - \frac{Hi}{6} (k \Delta x)^3 +  O( \Delta x^4) \]

\[\mathcal{D}\mathcal{F}^{h,h}_1 = -\frac{\sqrt{gH}}{ 2} k^2 \Delta x + O( \Delta x^3) \]
\[\mathcal{D}\mathcal{F}^{u,h}_1 = igHk -\frac{igHk^3(\Delta x)^2}{6} +  O( \Delta x^3) \]
\[\mathcal{D}\mathcal{F}^{u,u}_1 = \frac{i\sqrt{gH}H}{6}(H^2 + 3) k^2(\Delta x) - \frac{\sqrt{gH}H}{72}(2H^2 + 3)k^4 (\Delta x)^3 + O( \Delta x^5) \]


\section{Taylor Expansions Of Second Order Values }

\[\mathcal{G}_2 = H +\frac{H^3}{3} k^2 -\frac{H^3 k^4(\Delta x)^2}{36} + O(x^{4})\]

\[\mathcal{M}_2 = 1\]

\[\mathcal{R}_2^- = 1  + \frac{i}{2} (k \Delta x) - \frac{i}{12}(k \Delta x)^3  +  O(x^{4})\]

\[\mathcal{R}_2^+ =1 + \frac{i}{2}k\Delta x + \frac{i}{6} k^3 \Delta x^3 + O\left(\Delta x ^4\right)\]

\[\mathcal{R}^u_2 = 1 + \frac{i}{2}k\Delta x - \frac{1}{4} (k \Delta x)^2 - \frac{i}{12} (k \Delta x)^3 +  O( \Delta x^4)\]

\[\mathcal{D}\mathcal{F}_2^{h,u} = Hik - \frac{iH}{6}k^3(\Delta x)^2 + \frac{iH}{120}k^5 (\Delta x)^4 + O(\Delta x ^5) \]

\[\mathcal{D}\mathcal{F}_2^{h,h} = \frac{\sqrt{gH}}{8} k^4(\Delta x)^3  - \frac{\sqrt{gH}}{48} k^6(\Delta x)^5 + O(\Delta x^7) \]

\[\mathcal{D}\mathcal{F}_2^{u,u} =  \frac{\sqrt{gH}}{24}H(H^2 +3)k^4 \Delta x^3 - \frac{\sqrt{gH}}{96}H(H^2 +2)k^6 \Delta x^5 + O(\Delta x ^6)\]

\[\mathcal{D}\mathcal{F}_2^{u,h} = igHk + \frac{igH}{12}  k^3 \Delta x^2 - \frac{13igH}{240}  k^5 \Delta x^4 + O(\Delta x ^6)  \]

\section{Taylor Expansions Of Third Order Values }

\[\mathcal{G}_3 = H + \frac{H^3k^2}{3} -\frac{H^3 k^6 (\Delta x)^4}{270} + O(\Delta x^{6}) \]

\[\mathcal{M}_3= 1 + \frac{1}{24} (k\Delta x)^2 - \frac{1}{288} (k\Delta x)^4 + O(x^{6})\]

\[R_3^-= 1 + \frac{i}{2}k\Delta x - \frac{1}{24} (k \Delta x)^2 - \frac{1}{16} (k \Delta x)^3 +  O( \Delta x^4) \]

\[R_3^+= 1 + \frac{i}{2}k\Delta x - \frac{1}{24} (k \Delta x)^2 - \frac{5}{48} (k \Delta x)^3 +  O( \Delta x^4)\] 

\[R^u_3 = 1 + \frac{i}{2}k\Delta x - \frac{1}{8} (k \Delta x)^2 - \frac{i}{48} (k \Delta x)^3 +  O( \Delta x^4) \]

\[\mathcal{D}\mathcal{F}_3^{h,u} = iHk - \frac{iH}{24} k^3 \Delta x ^2 - \frac{11iH}{480 }k^5 \Delta x ^4 + O(\Delta x ^6) \]

\[\mathcal{D}\mathcal{F}_3^{h,h} = \frac{\sqrt{gH}}{12} k^4 \Delta x^3 - \frac{\sqrt{gH}}{96}k^6 \Delta x^5 + \frac{\sqrt{gH}}{5760}k^8 \Delta x^7 + O(\Delta x ^8)\]

\[\mathcal{D}\mathcal{F}_3^{u,u} = \frac{\sqrt{gH}}{12}(\frac{H^3}{3} + H) k^4 \Delta x^3 - \frac{\sqrt{gH}}{96}(\frac{H^3}{3} + H)k^6 \Delta x^5  + O(\Delta x ^7)\]

\[\mathcal{D}\mathcal{F}_3^{u,h} = igH k + \frac{igH}{24} k^3 \Delta x^2 - \frac{-53 igH }{1440} k^5\Delta x^4 + O(\Delta x ^6) \]
\end{document}
